Remove unnecessary admits

Scratch.v
@@ -1,26 +1,14 @@
-Require Import Utf8.
-Require Import Setoid.
+Definition eq {A} (x y : A) :=
+  forall P : A -> Prop, P x -> P y.
 
-Axiom neg_conj : ∀ P Q, ¬(P /\ Q) <-> ¬P \/ ¬Q.
-Axiom neg_disj : ∀ P Q, ¬(P \/ Q) <-> ¬P /\ ¬Q.
-Axiom neg_forall : ∀ A (P : A -> Prop), ¬(∀ x, P x) <-> ∃ x, ¬P x.
-Axiom neg_exists : ∀ A (P : A -> Prop), ¬(∃ x, P x) <-> ∀ x, ¬P x.
-Axiom neg_neg : ∀ P : Prop, ¬¬P <-> P.
-Axiom neg_impl : ∀ P Q : Prop, ¬(P -> Q) <-> (P /\ ¬Q).
+Context {A : Type}.
 
-Ltac negate H :=
-  repeat (
-    setoid_rewrite neg_neg in H ||
-    setoid_rewrite neg_conj in H ||
-    setoid_rewrite neg_disj in H ||
-    setoid_rewrite neg_impl in H ||
-    setoid_rewrite neg_forall in H ||
-    setoid_rewrite neg_exists in H
-  ).
+Theorem eq_refl : forall x : A, eq x x.
+Proof. easy. Qed.
 
-Parameter P Q R : Prop.
-
-Goal ¬(¬¬(¬P /\ (R -> ¬(P /\ Q))) /\ Q) → False.
+Theorem eq_symm : forall x y : A, eq x y -> eq y x.
 Proof.
-  intros.
-  negate H.
+  unfold eq. intros.
+  specialize (H (fun z => P z -> P x) (fun x => x)).
+  now apply H.
+Qed.
